Support functions without return statements in the frontend.
We achieve this by inserting a dummy return at the end when needed.

tests/defined/no_return.c
@@ -1,0 +1,7 @@
+int f() {
+  if(1) return 10;
+}
+
+int main() {
+  printf("%d\n", f());
+}
